Consider a function safetail that behaves in the same way as tail, except that safetail maps the empty list to the empty list, whereas tail gives an error in this case.  
â€¢Define safetail using:
1. A conditional expression
2. Guarded equations
3. Pattern matching


```haskell
safetail' :: [a] -> [a]
safetail' xs = if null xs then xs else tail xs

safetail'' :: [a] -> [a]
safetail'' xs | null xs    = xs
              | otherwise  = tail xs

safetail''' ::  [a] -> [a]
safetail''' [] = []
safetail''' (_:xs) = xs

```